Translation/Entry.lean
@@ -1,0 +1,14 @@
+import Surface.Global
+import Core.Global
+
+import Translation.Ty
+import Translation.Term
+
+
+def Surface.Entry.translate : Surface.Entry -> Core.Entry
+| data x K ctors => .data x K.translate ((λ x => (x.1 , x.2.translate)) <$>ctors)
+| ctor x i T => .ctor x i T.translate
+| opent x K => .opent x K.translate
+| openm x T => .openm x T.translate
+
+notation "⟦" e "⟧" => Surface.Entry.translate e
