Translation/Entry/Lemmas.lean
@@ -1,0 +1,2 @@
+import Translation.Entry
+import Translation.Global
